isabelle/Doc/Specification/SpecificationLatexSugar.thy
@@ -1,0 +1,21 @@
+theory SpecificationLatexSugar 
+imports "HOL-Library.LaTeXsugar"
+begin 
+
+(* By default all thm exports should use the names_short property. This can be switched on a 
+thm by thm basis. *)
+declare [[ names_short ]]
+
+
+(* Display lists more closely to Haskell syntax *)
+
+notation (latex)
+  Cons  ("_ :/ _" [66,65] 65)
+
+syntax (latex output)
+  "_appendL" :: "'a list \<Rightarrow> 'a list \<Rightarrow> 'a list" (infixl "\<^latex>\<open>++\<close>" 65)
+
+translations
+  "_appendL xs ys" <= "xs @ ys" 
+  "_appendL (_appendL xs ys) zs" <= "_appendL xs (_appendL ys zs)"
+end 
